read_mem_aux contract for block verifier

src/verification/BlockVer/Spec.v
@@ -33,6 +33,10 @@ Open Scope ctx_scope.
 Open Scope Z_scope.
 
 Module Assembly.
+  Definition MPUIPC0_addr {Σ} : Term Σ _ := term_val ty.Address [bv 0x05AA].
+  Definition MPUIPSEGB2_addr {Σ} : Term Σ _ := term_val ty.Address [bv [16] 0x05AC].
+  Definition MPUIPSEGB1_addr {Σ} : Term Σ _ := term_val ty.Address [bv [16] 0x05AE].
+
   Inductive ast_with_args :=
   | I0 (i : ast)
   | I1 (i : ast) (a : bv 16)
@@ -72,28 +76,35 @@ Module Assembly.
       (DOUBLEOP MOV WORD_INSTRUCTION rs INDEXED_MODE rd INDIRECT_REGISTER_MODE)
       i.
 
+  Definition mov_ir rs i rd :=
+    I1
+      (DOUBLEOP MOV WORD_INSTRUCTION rs INDEXED_MODE rd REGISTER_MODE)
+      i.
+
   Definition xor_ar rs rd :=
     I0 (DOUBLEOP XOR WORD_INSTRUCTION rs INDIRECT_AUTOINCREMENT_MODE rd REGISTER_MODE).
 
+  Definition jump kind off :=
+    I0 (JUMP kind off).
+
 End Assembly.
 
-Module MSP430BlockVerifSpec <: Specification MSP430Base MSP430Signature MSP430Program.
-  Include SpecificationMixin MSP430Base MSP430Signature MSP430Program.
-
+Module Utils.
   Import asn.notations.
+  Import Assembly.
 
-  Local Notation "a @ b" := (term_binop (@bop.bvapp _ 8 8) a b) (at level 60).
-  Local Notation "v +' n" :=  (term_binop bop.bvadd v (term_val ty.wordBits [bv n])) (at level 50).
+  Notation "a @ b" := (term_binop (@bop.bvapp _ 8 8) a b) (at level 60).
+  Notation "v +' n" :=  (term_binop bop.bvadd v (term_val ty.wordBits [bv n])) (at level 50).
 
-  Local Notation "a m↦ v" := (asn.chunk (chunk_user ptstomem [a; v])) (at level 70).
-  Local Notation "a i↦ i" := (asn.chunk (chunk_user ptstoinstr [a; i])) (at level 70).
-  Local Notation "w ≡ i" := (asn.chunk (chunk_user encodes_instr [w; i])) (at level 70).
+  Notation "a m↦ v" := (asn.chunk (chunk_user ptstomem [a; v])) (at level 70).
+  Notation "a i↦ i" := (asn.chunk (chunk_user ptstoinstr [a; i])) (at level 70).
+  Notation "w ≡ i" := (asn.chunk (chunk_user encodes_instr [w; i])) (at level 70).
 
-  Local Notation asn_accessible_addresses segb1 segb2 :=
+  Notation asn_accessible_addresses segb1 segb2 :=
     (asn.chunk_angelic (chunk_user accessible_addresses
                           [term_var segb1; term_var segb2])).
 
-  Local Notation asn_accessible_addresses_without segb1 segb2 addr :=
+  Notation asn_accessible_addresses_without segb1 segb2 addr :=
     (asn.chunk_angelic (chunk_user accessible_addresses_without
                           [term_var segb1; term_var segb2; term_var addr])).
 
@@ -105,6 +116,25 @@ Module MSP430BlockVerifSpec <: Specification MSP430Base MSP430Signature MSP430Pr
        (term_unsigned w)
        (term_val ty.int 16%Z)).
 
+  Definition high {Σ} (v : Term Σ (ty.bvec 16)) : Term Σ _ := term_vector_subrange 0 8 v.
+  Definition low {Σ} (v : Term Σ (ty.bvec 16)) : Term Σ _ := term_vector_subrange 8 8 v.
+
+  Definition bor1 {Σ} (v : Term Σ ty.wordBits) : Term Σ _ :=
+    term_binop bop.bvor v (term_val ty.wordBits [bv 1]).
+
+  Definition asn_word_aligned {Σ} (addr : Term Σ ty.Address) : Assertion Σ :=
+    addr = term_binop bop.bvand addr (term_val ty.Address [bv 0xfffe]).
+
+  Definition asn_ptsto_word {Σ}
+    (addr : Term Σ ty.Address)
+    (bl bh : Term Σ ty.byteBits)
+    : Assertion Σ
+  :=
+      addr m↦ bl
+    ∗ bor1 addr m↦ bh.
+
+  Notation "a w↦ l h" := (asn_ptsto_word a l h) (at level 70).
+
   Definition asn_ipe_entry_point {Σ}
       (segb1 addr : Term Σ ty.wordBits)
       : Assertion Σ
@@ -114,21 +144,9 @@ Module MSP430BlockVerifSpec <: Specification MSP430Base MSP430Signature MSP430Pr
            (term_plus 8 (word_times_16 segb1))
            (term_unsigned addr)).
 
-  Definition asn_unprotected {Σ}
-      (segb1 segb2 : Term Σ ty.wordBits)
-      (am : Term Σ (ty.enum Eaccess_mode))
-      (addr : Term Σ ty.Address)
-      : Assertion Σ
-    :=
-        asn.formula (formula_relop bop.lt
-                       (term_unsigned addr)
-                       (word_times_16 segb1))
-      ∨ asn.formula (formula_relop bop.le
-                       (word_times_16 segb2)
-                       (term_unsigned addr))
-
-      ∨ ( am = term_enum Eaccess_mode X
-        ∗ asn_ipe_entry_point segb1 addr).
+  Definition asn_not_mpu_reg_addr {Σ} (addr : Term Σ ty.Address) : Assertion Σ :=
+    term_unsigned addr < term_unsigned MPUIPC0_addr
+    ∨ term_unsigned (MPUIPSEGB1_addr +' 2) <= term_unsigned addr.
 
   Definition asn_mpu_registers {Σ} : Assertion Σ :=
       ∃ "MPUCTL0_reg"    , MPUCTL0_reg    ↦ term_var "MPUCTL0_reg"
@@ -136,6 +154,14 @@ Module MSP430BlockVerifSpec <: Specification MSP430Base MSP430Signature MSP430Pr
     ∗ ∃ "MPUSEGB2_reg"   , MPUSEGB2_reg   ↦ term_var "MPUSEGB2_reg"
     ∗ ∃ "MPUSEGB1_reg"   , MPUSEGB1_reg   ↦ term_var "MPUSEGB1_reg"
     ∗ ∃ "MPUSAM_reg"     , MPUSAM_reg     ↦ term_var "MPUSAM_reg".
+End Utils.
+
+Module MSP430BlockVerifSpec <: Specification MSP430Base MSP430Signature MSP430Program.
+  Include SpecificationMixin MSP430Base MSP430Signature MSP430Program.
+
+  Import asn.notations.
+  Import Assembly.
+  Import Utils.
 
   Definition SepContractFun {Δ τ} (f : Fun Δ τ) : Type :=
     SepContract Δ τ.
@@ -150,8 +176,8 @@ Module MSP430BlockVerifSpec <: Specification MSP430Base MSP430Signature MSP430Pr
 
   Definition lemma_extract_accessible_ptsto : SepLemma extract_accessible_ptsto :=
     {|
-      lemma_logic_variables := ["addr" :: ty.Address; "m" :: ty.enum Eaccess_mode];
-      lemma_patterns := [term_var "addr"; term_var "m"];
+      lemma_logic_variables := ["addr" :: ty.Address];
+      lemma_patterns := [term_var "addr"];
       lemma_precondition := ⊤;
       lemma_postcondition := ⊤;
     |}.
@@ -172,39 +198,29 @@ Module MSP430BlockVerifSpec <: Specification MSP430Base MSP430Signature MSP430Pr
       lemma_precondition    := term_var "addr" i↦ term_var "id";
       lemma_postcondition   :=
         ∃ "bl", ∃ "bh",
-
-        ( ∃ "i",
-            (term_var "id" = term_union Uinstr_or_data Ki (term_var "i")
-             ∗ term_var "addr" m↦ term_var "bl"
-             ∗ term_var "addr" +' 1 m↦ term_var "bh"
-             ∗ term_var "bh" @ term_var "bl" ≡ term_var "i")
-
-        ∨
-
-         ∃ "d",
-           (term_var "id" = term_union Uinstr_or_data Kd (term_var "d")
-            ∗ term_var "addr" m↦ term_var "bl"
-            ∗ term_var "addr" +' 1 m↦ term_var "bh"
-            ∗ term_var "bh" @ term_var "bl" = term_var "d"))
+        ( asn_ptsto_word (term_var "addr") (term_var "bl") (term_var "bh")
+        ∗ ( ∃ "i", (term_var "id" = term_union Uinstr_or_data Ki (term_var "i")
+                    ∗ term_var "bh" @ term_var "bl" ≡ term_var "i")
+          ∨ ∃ "d", (term_var "id" = term_union Uinstr_or_data Kd (term_var "d")
+                    ∗ term_var "bh" @ term_var "bl" = term_var "d")))
     |}.
 
   Definition lemma_close_ptsto_instr : SepLemma close_ptsto_instr :=
     {|
       lemma_logic_variables :=
-        [ "addr" :: ty.wordBits; "i" :: ty.union Uast
-        ; "bl" :: ty.byteBits; "bh" :: ty.byteBits
-        ];
+        [ "addr" :: ty.wordBits; "id" :: ty.union Uinstr_or_data ];
 
-      lemma_patterns := [term_var "addr"(* ; term_var "w" *)];
+      lemma_patterns := [term_var "addr"];
 
-      lemma_precondition := ⊤;
-        (*   term_var "addr" m↦ term_var "bl" *)
-        (* ∗ term_binop bop.bvadd (term_var "addr") (term_val ty.wordBits [bv 1]) *)
-        (*     m↦ term_var "bh" *)
-        (* ∗ term_binop (@bop.bvapp _ 8 8) (term_var "bh") (term_var "bl") *)
-        (*     ≡ term_var "i"; *)
+      lemma_precondition :=
+        ∃ "bl", ∃ "bh",
+        ( asn_ptsto_word (term_var "addr") (term_var "bl") (term_var "bh")
+        ∗ ( ∃ "i", (term_var "id" = term_union Uinstr_or_data Ki (term_var "i")
+                    ∗ term_var "bh" @ term_var "bl" ≡ term_var "i")
+          ∨ ∃ "d", (term_var "id" = term_union Uinstr_or_data Kd (term_var "d")
+                    ∗ term_var "bh" @ term_var "bl" = term_var "d")));
 
-      lemma_postcondition := (* term_var "addr" i↦ term_var "i" *) ⊤;
+      lemma_postcondition := term_var "addr" i↦ term_var "id";
     |}.
 
   (* Foreign function contracts *)
@@ -244,56 +260,6 @@ Module MSP430BlockVerifSpec <: Specification MSP430Base MSP430Signature MSP430Pr
         ∗ term_var "u" = term_val ty.unit tt;
     |}.
 
-  (* Sail function contracts *)
-
-  Definition sep_contract_fetch : SepContractFun fetch :=
-    {|
-      sep_contract_logic_variables :=
-        [ "ipectl" :: ty.wordBits; "segb1" :: ty.wordBits; "segb2" :: ty.wordBits
-        ; "pc_old" :: ty.wordBits; "id" :: ty.union Uinstr_or_data
-        ; "u" :: ty.unit ];
-
-      sep_contract_localstore := [ term_var "u" ];
-
-      sep_contract_precondition :=
-          PC_reg         ↦ term_var "pc_old"
-        ∗ MPUIPC0_reg    ↦ term_var "ipectl"
-        ∗ MPUIPSEGB1_reg ↦ term_var "segb1"
-        ∗ MPUIPSEGB2_reg ↦ term_var "segb2"
-        ∗ asn_mpu_registers
-
-        (* ∗ asn_ipe_configured  (term_var "ipectl") *)
-        (* ∗ asn_untrusted *)
-        (*     (term_var "segb1") (term_var "segb2") (term_var "pc_old") *)
-
-        ∗ term_var "pc_old" i↦ term_var "id";
-
-      sep_contract_result          := "v";
-      sep_contract_postcondition   :=
-          MPUIPC0_reg    ↦ term_var "ipectl"
-        ∗ MPUIPSEGB1_reg ↦ term_var "segb1"
-        ∗ MPUIPSEGB2_reg ↦ term_var "segb2"
-        ∗ asn_mpu_registers
-
-        ∗ PC_reg ↦ term_var "pc_old" +' 2
-
-        ∗ term_var "pc_old" i↦ term_var "id"
-        ∗ ∃ "w",
-          ( term_var "v" = term_union Uwordbyte Kword (term_var "w")
-
-          ∗ ( ∃ "i", ( term_var "id" = term_union Uinstr_or_data Ki (term_var "i")
-                     ∗ term_var "w" ≡ term_var "i")
-            ∨ term_var "id" = term_union Uinstr_or_data Kd (term_var "w")));
-
-      (* encodes_instr is duplicable *)
-
-        (* ∗ ∃ "pc_new", *)
-        (*   ( term_var "pc_new" = term_word_plus [bv 2] (term_var "pc_old") *)
-        (*     ∗ PC_reg ↦ term_var "pc_new" *)
-        (*     ∗ asn_untrusted *)
-        (*         (term_var "segb1") (term_var "segb2") (term_var "pc_new")); *)
-    |}.
-
   Definition sep_contract_decode : SepContractFunX decode :=
     {|
       sep_contract_logic_variables :=
@@ -308,11 +274,173 @@ Module MSP430BlockVerifSpec <: Specification MSP430Base MSP430Signature MSP430Pr
       sep_contract_postcondition   := term_var "r" = term_var "i";
     |}.
 
+  (* Sail function contracts *)
+
+  (*
+  Definition asn_read_mpu_reg_result {Σ}
+    (ipectl segb1 segb2 addr : Term Σ ty.wordBits) (v : Term Σ ty.byteBits)
+    : Assertion Σ
+  :=
+    ( addr = MPUIPC0_addr ∗ v = low ipectl
+    ∨ addr = MPUIPC0_addr +' 1 ∗ v = high ipectl
+    ∨ addr = MPUIPSEGB1_addr ∗ v = low segb1
+    ∨ addr = MPUIPSEGB1_addr +' 1 ∗ v = high segb1
+    ∨ addr = MPUIPSEGB2_addr ∗ v = low segb2
+    ∨ addr = MPUIPSEGB2_addr +' 1 ∗ v = high segb2
+    ∨ term_unsigned addr < term_unsigned MPUIPC0_addr
+    ∨ term_unsigned (MPUIPSEGB1_addr +' 2) <= term_unsigned addr).
+
+  Definition sep_contract_read_mpu_reg_byte :
+    SepContractFun read_mpu_reg_byte :=
+    {|
+      sep_contract_logic_variables :=
+        [ "addr" :: ty.Address; "ipectl" :: ty.wordBits
+        ; "segb1" :: ty.wordBits; "segb2" :: ty.wordBits ];
+
+      sep_contract_localstore := [term_var "addr"];
+
+      sep_contract_precondition :=
+          MPUIPC0_reg    ↦ term_var "ipectl"
+        ∗ MPUIPSEGB1_reg ↦ term_var "segb1"
+        ∗ MPUIPSEGB2_reg ↦ term_var "segb2"
+        ∗ asn_mpu_registers;
+
+      sep_contract_result        := "v";
+      sep_contract_postcondition :=
+          asn_read_mpu_reg_result
+            (term_var "ipectl") (term_var "segb1") (term_var "segb2")
+            (term_var "addr") (term_var "v")
+
+        ∗ MPUIPC0_reg    ↦ term_var "ipectl"
+        ∗ MPUIPSEGB1_reg ↦ term_var "segb1"
+        ∗ MPUIPSEGB2_reg ↦ term_var "segb2"
+        ∗ asn_mpu_registers;
+    |}.
+   *)
+
+  Definition sep_contract_check_byte_access :
+    SepContractFun check_byte_access :=
+    {|
+      sep_contract_logic_variables :=
+        [ "addr" :: ty.Address; "jump" :: ty.bool
+        ; "pc" :: ty.wordBits; "ipectl" :: ty.wordBits
+        ; "segb1" :: ty.wordBits; "segb2" :: ty.wordBits
+        ];
+
+      sep_contract_localstore := [term_var "addr"; term_var "jump"];
+
+      sep_contract_precondition :=
+          PC_reg         ↦ term_var "pc"
+        ∗ MPUIPC0_reg    ↦ term_var "ipectl"
+        ∗ MPUIPSEGB1_reg ↦ term_var "segb1"
+        ∗ MPUIPSEGB2_reg ↦ term_var "segb2";
+
+      sep_contract_result        := "v";
+      sep_contract_postcondition :=
+          term_var "v" = term_val ty.unit tt
+
+        ∗ PC_reg         ↦ term_var "pc"
+        ∗ MPUIPC0_reg    ↦ term_var "ipectl"
+        ∗ MPUIPSEGB1_reg ↦ term_var "segb1"
+        ∗ MPUIPSEGB2_reg ↦ term_var "segb2";
+    |}.
+
+  Definition sep_contract_read_mem_aux :
+      SepContractFun read_mem_aux :=
+      {|
+        sep_contract_logic_variables :=
+          [ "bw" :: ty.enum Ebw; "addr" :: ty.Address; "pc" :: ty.wordBits
+          ; "ipectl" :: ty.wordBits; "segb1" :: ty.wordBits; "segb2" :: ty.wordBits
+          ; "bl" :: ty.byteBits; "bh" :: ty.byteBits ];
+
+        sep_contract_localstore := [term_var "bw"; term_var "addr"];
+
+        sep_contract_precondition :=
+            PC_reg         ↦ term_var "pc"
+          ∗ MPUIPC0_reg    ↦ term_var "ipectl"
+          ∗ MPUIPSEGB1_reg ↦ term_var "segb1"
+          ∗ MPUIPSEGB2_reg ↦ term_var "segb2"
+
+          ∗ ( ( term_var "bw" = term_enum Ebw WORD_INSTRUCTION
+              ∗ asn_ptsto_word (term_var "addr") (term_var "bl") (term_var "bh")
+              (* ∗ asn_word_aligned (term_var "addr") *))
+            ∨ ( term_var "bw" = term_enum Ebw BYTE_INSTRUCTION
+              ∗ term_var "addr" m↦ term_var "bl"))
+
+          (* the bootcode never reads the MPU registers *)
+          ∗ asn_not_mpu_reg_addr (term_var "addr");
+
+        sep_contract_result        := "v";
+        sep_contract_postcondition :=
+            ( ( term_var "bw" = term_enum Ebw WORD_INSTRUCTION
+              ∗ term_var "v" = term_union Uwordbyte Kword (term_var "bh" @ term_var "bl")
+              ∗ asn_ptsto_word (term_var "addr") (term_var "bl") (term_var "bh"))
+            ∨ ( term_var "bw" = term_enum Ebw BYTE_INSTRUCTION
+              ∗ term_var "v" = term_union Uwordbyte Kbyte (term_var "bl")
+              ∗ term_var "addr" m↦ term_var "bl"))
+
+          ∗ PC_reg         ↦ term_var "pc"
+          ∗ MPUIPC0_reg    ↦ term_var "ipectl"
+          ∗ MPUIPSEGB1_reg ↦ term_var "segb1"
+          ∗ MPUIPSEGB2_reg ↦ term_var "segb2";
+      |}.
+
+  (* Definition sep_contract_fetch : SepContractFun fetch := *)
+  (*   {| *)
+  (*     sep_contract_logic_variables := *)
+  (*       [ "ipectl" :: ty.wordBits; "segb1" :: ty.wordBits; "segb2" :: ty.wordBits *)
+  (*       ; "pc_old" :: ty.wordBits; "id" :: ty.union Uinstr_or_data *)
+  (*       ; "u" :: ty.unit ]; *)
+
+  (*     sep_contract_localstore := [ term_var "u" ]; *)
+
+  (*     sep_contract_precondition := *)
+  (*       term_var "pc_old" = term_val ty.wordBits [bv 0] ∗ *)
+  (*         PC_reg         ↦ term_var "pc_old" *)
+  (*       ∗ MPUIPC0_reg    ↦ term_var "ipectl" *)
+  (*       ∗ MPUIPSEGB1_reg ↦ term_var "segb1" *)
+  (*       ∗ MPUIPSEGB2_reg ↦ term_var "segb2" *)
+  (*       ∗ asn_mpu_registers *)
+
+  (*       (* ∗ asn_ipe_configured  (term_var "ipectl") *) *)
+  (*       (* ∗ asn_untrusted *) *)
+  (*       (*     (term_var "segb1") (term_var "segb2") (term_var "pc_old") *) *)
+
+  (*       ∗ term_var "pc_old" i↦ term_var "id"; *)
+
+  (*     sep_contract_result          := "v"; *)
+  (*     sep_contract_postcondition   := *)
+  (*         MPUIPC0_reg    ↦ term_var "ipectl" *)
+  (*       ∗ MPUIPSEGB1_reg ↦ term_var "segb1" *)
+  (*       ∗ MPUIPSEGB2_reg ↦ term_var "segb2" *)
+  (*       (* ∗ asn_mpu_registers *) *)
+
+  (*       (* ∗ PC_reg ↦ term_var "pc_old" +' 2 *) *)
+
+  (*       (* ∗ term_var "pc_old" i↦ term_var "id" *) *)
+  (*       (* ∗ ∃ "w", *) *)
+  (*       (*   ( term_var "v" = term_union Uwordbyte Kword (term_var "w") *) *)
+
+  (*       (*   ∗ ( ∃ "i", ( term_var "id" = term_union Uinstr_or_data Ki (term_var "i") *) *)
+  (*       (*              ∗ term_var "w" ≡ term_var "i") *) *)
+  (*       (*     ∨ term_var "id" = term_union Uinstr_or_data Kd (term_var "w"))) *); *)
+
+  (*     (* encodes_instr is duplicable *) *)
+
+  (*       (* ∗ ∃ "pc_new", *) *)
+  (*       (*   ( term_var "pc_new" = term_word_plus [bv 2] (term_var "pc_old") *) *)
+  (*       (*     ∗ PC_reg ↦ term_var "pc_new" *) *)
+  (*       (*     ∗ asn_untrusted *) *)
+  (*       (*         (term_var "segb1") (term_var "segb2") (term_var "pc_new")); *) *)
+  (*   |}. *)
 
   Definition CEnv : SepContractEnv :=
     fun Δ τ f =>
       match f with
-      | fetch => Some sep_contract_fetch
+      | read_mem_aux => Some sep_contract_read_mem_aux
+      (* | write_mpu_reg_byte => Some sep_contract_write_mpu_reg_byte *)
+      | check_byte_access => Some sep_contract_check_byte_access
+      (* | fetch => Some sep_contract_fetch *)
       | _ => None
       end.
 
@@ -339,3 +467,35 @@ Module MSP430BlockVerifShalExecutor :=
   MakeShallowExecutor MSP430Base MSP430Signature MSP430Program MSP430BlockVerifSpec.
 Module MSP430BlockVerifExecutor :=
   MakeExecutor MSP430Base MSP430Signature MSP430Program MSP430BlockVerifSpec.
+
+Module RiscvPmpSpecVerif.
+  Import MSP430BlockVerifSpec.
+  Import MSP430BlockVerifExecutor.Symbolic.
+  Import MSP430BlockVerifExecutor.
+
+  Import ModalNotations.
+  Import Erasure.notations.
+
+  Ltac symbolic_simpl :=
+    apply validcontract_with_erasure_and_fuel_sound;
+    compute;
+    constructor;
+    simpl.
+
+  Definition ValidContractWithFuel {Δ τ} (fuel : nat) (c : SepContract Δ τ) (body : Stm Δ τ) : Prop :=
+  VerificationCondition
+    ((SPureSpec.replay ( (vcgen default_config fuel c body wnil)))).
+  
+  Lemma valid_read_mem_aux : ValidContractWithFuel 10 sep_contract_read_mem_aux fun_read_mem_aux.
+  Proof.
+  vm_compute. Set Printing Depth 200. Admitted.
+    (* symbolic_simpl. Admitted. *)
+
+  Lemma valid_check_byte_access : ValidContractWithFuel 10 sep_contract_check_byte_access fun_check_byte_access.
+  Proof. now symbolic_simpl. Qed.
+
+  (* Lemma valid_execute_fetch : ValidContractWithFuel 10 sep_contract_fetch fun_fetch. *)
+  (* Proof. *)
+  (*   symbolic_simpl. *)
+  (* Qed. *)
+End RiscvPmpSpecVerif.
